attention progress

src/lib/kernel/Kuiper.Kernel.Attention.fst
@@ -9,23 +9,42 @@ open Kuiper.Tensor
 open Kuiper.Index
 open Kuiper.Bijection
 
-open Kuiper.Spec.Attention
-
 module EM4 = Kuiper.EMatrix4
 module EM3 = Kuiper.EMatrix3
 module CH = Kuiper.Chest
 module SZ = Kuiper.SizeT
 
+open Kuiper.Spec.Attention
+open Kuiper.Kernel.BatchedGEMM
 
+
+#push-options "--split_queries always"
+let transpose4_2 (#d0 #d1 #d2 #d3 : nat) : 
+  (abs (d0 @| d1 @| d2 @| d3 @| INil) =~ abs (d0 @| d1 @| d3 @| d2 @| INil)) =
+{
+  ff = (fun (i,(j,(k,(l,())))) -> (i,(j,(l,(k,())))));
+  gg = (fun (i,(j,(k,(l,())))) -> (i,(j,(l,(k,())))));
+  // weird that ez doesn't take care of it...
+  ff_gg = (fun x -> (
+    let (i,(j,(k,(l,())))) = x in
+    assert ((fun (i,(j,(k,(l,())))) -> (i,(j,(l,(k,()))))) x) == (i,(j,(l,(k,()))))
+  ));
+  gg_ff = (fun x -> (
+    let (i,(j,(k,(l,())))) = x in
+    assert ((fun (i,(j,(k,(l,())))) -> (i,(j,(l,(k,()))))) x) == (i,(j,(l,(k,()))))
+  ));
+}
+
+//#push-options "--print_implicits"
 fn scaled_dot_product_efficient_attention
   (#et : Type0) {| floating et, real_like et, floating_real_like et |}
   (n h : szp)
   (l s : szp)
   (e ev : szp)
-  (#lQ: tlayout    (n @| h @| l @| e @| INil))
-  (#lK: tlayout    (n @| h @| s @| e @| INil))
-  (#lV: tlayout    (n @| h @| s @| ev @| INil))
-  (#lbias: tlayout (n @| h @| l @| s @| INil))
+  (#lQ: tlayout    (n @| h @| l @| e @| INil) { is_full lQ }) // needed for tlayout_bij for now.
+  (#lK: tlayout    (n @| h @| s @| e @| INil) { is_full lK })
+  (#lV: tlayout    (n @| h @| s @| ev @| INil) { is_full lV })
+  (#lbias: tlayout (n @| h @| l @| s @| INil) { is_full lbias })
   {| ctlayout lQ, ctlayout lK, ctlayout lV, ctlayout lbias |}
   (gQ    : tensor et lQ    { is_global gQ    })
   (gK    : tensor et lK    { is_global gK    })
@@ -73,6 +92,54 @@ fn scaled_dot_product_efficient_attention
             (to_real scale) in
           eO %~ out_spec /\ eLSE %~ lse_spec)) **
     pure (is_global (fst out) /\ is_global (snd out)) {
+
+  map_loc gpu_loc (fun () -> tensor_pts_to_ref gQ);
+  map_loc gpu_loc (fun () -> tensor_pts_to_ref gK);
+  map_loc gpu_loc (fun () -> tensor_pts_to_ref gV);
+  map_loc gpu_loc (fun () -> tensor_pts_to_ref gbias);
+  
+  let rQ = EM4.to_real_matrix eQ;
+  let rV = EM4.to_real_matrix eV;
+  let rbias = EM3.to_real_matrix ebias;
+
+  // Transpose K via ghost
+  let f_transpose = transpose4_2 #n #h #s #e; 
+  let gKT: tensor et (tlayout_bij f_transpose lK) = from_array (tlayout_bij f_transpose lK) (core gK);
+  assert rewrites_to gKT (from_array (tlayout_bij f_transpose lK) (core gK));
+  map_loc gpu_loc (fun () -> tensor_apply_bij f_transpose gK #fK);
+  let eKT = CH.mk (n @| h @| e @| s @| INil) (fun i -> CH.acc eK (i <~| f_transpose));
+  assert on gpu_loc (gKT |-> Frac fK eKT);
+  assert pure (eKT %~ rKT);
+
+  // Fold 2 batch dimensions of K^T, Q, V into one (N * H)
+  let gKTf = from_array (tlayout_fold_outer (tlayout_bij f_transpose lK)) (core gKT);
+  let gQf = from_array (tlayout_fold_outer lQ) (core gQ);
+  let gVf = from_array (tlayout_fold_outer lV) (core gV);
+  let gbiasf = from_array (tlayout_fold_outer lbias) (core gbias);
+  assert rewrites_to gKTf (from_array (tlayout_fold_outer (tlayout_bij f_transpose lK)) (core gKT));
+  assert rewrites_to gQf (from_array (tlayout_fold_outer lQ) (core gQ));
+  assert rewrites_to gVf (from_array (tlayout_fold_outer lV) (core gV));
+  assert rewrites_to gbiasf (from_array (tlayout_fold_outer lbias) (core gbias));
+  
+  map_loc gpu_loc (fun () -> tensor_fold_outer gQ #fQ);
+  map_loc gpu_loc (fun () -> tensor_fold_outer gV #fV);
+  map_loc gpu_loc (fun () -> tensor_fold_outer gKT #fK);
+  map_loc gpu_loc (fun () -> tensor_fold_outer gbias #fbias);
+
+  let eQf = fold_chest eQ; 
+  let eVf = fold_chest eV; 
+  let eKTf = fold_chest eKT; 
+  let ebiasf = fold_chest ebias;
+  assert on gpu_loc (gQf |-> Frac fQ eQf) ** pure (eQf %~ fold_chest rQ);
+  assert on gpu_loc (gVf |-> Frac fV eVf) ** pure (eVf %~ fold_chest rV);
+  assert on gpu_loc (gKTf |-> Frac fK eKTf) ** pure (eKTf %~ fold_chest rKT);
+  assert on gpu_loc (gbiasf |-> Frac fbias ebiasf) ** pure (ebiasf %~ fold_chest rbias);
+  
+  let gS = alloc0 #et (n *^ h *^ l *^ s) (l3_batched_row_major (n*^h) l s);
+  with eS. assert on gpu_loc (gS |-> eS);
+
+  bmmcomb_gpu_exact #et (fun bias_qk score -> (bias_qk +. score) *. scale) 
+    (n*^h) l e s gQf gKTf gS;
 
   admit ();
 }
